Globally rename `{DA,NA}.Finite` to `{DA,NA}.FinAcc`

Cslib/Computability/Automata/DAToNA.lean
@@ -26,18 +26,18 @@ def toNA (a : DA State Symbol) : NA State Symbol :=
 instance : Coe (DA State Symbol) (NA State Symbol) where
   coe := toNA
 
-namespace Finite
+namespace FinAcc
 
-/-- `DA.Finite` is a special case of `NA.Finite`. -/
+/-- `DA.FinAcc` is a special case of `NA.FinAcc`. -/
 @[scoped grind =]
-def toNAFinite (a : DA.Finite State Symbol) : NA.Finite State Symbol :=
+def toNAFinAcc (a : DA.FinAcc State Symbol) : NA.FinAcc State Symbol :=
   { a.toNA with accept := a.accept }
 
-open scoped Acceptor FLTS NA.Finite in
+open scoped Acceptor FLTS NA.FinAcc in
 /-- The `NA` constructed from a `DA` has the same language. -/
 @[scoped grind =]
-theorem toNAFinite_language_eq {a : DA.Finite State Symbol} :
-    Acceptor.language a = Acceptor.language a.toNAFinite := by
+theorem toNAFinAcc_language_eq {a : DA.FinAcc State Symbol} :
+    Acceptor.language a = Acceptor.language a.toNAFinAcc := by
   ext xs
   constructor
   · intro _
@@ -45,7 +45,7 @@ theorem toNAFinite_language_eq {a : DA.Finite State Symbol} :
     grind
   · grind
 
-end Finite
+end FinAcc
 
 end NA
 
